theories/autosubst/AST.v
@@ -9,7 +9,7 @@ Inductive term : Type :=
   | var : nat -> term
   | Sort : mode -> level -> term
   | Pi : mode -> mode -> term -> term -> term
-  | lam : term -> term -> term
+  | lam : mode -> term -> term -> term
   | app : term -> term -> term
   | Erased : term -> term
   | erase : term -> term
@@ -40,11 +40,13 @@ exact (eq_trans
          (ap (fun x => Pi t0 t1 t2 x) H3)).
 Qed.
 
-Lemma congr_lam {s0 : term} {s1 : term} {t0 : term} {t1 : term}
-  (H0 : s0 = t0) (H1 : s1 = t1) : lam s0 s1 = lam t0 t1.
+Lemma congr_lam {s0 : mode} {s1 : term} {s2 : term} {t0 : mode} {t1 : term}
+  {t2 : term} (H0 : s0 = t0) (H1 : s1 = t1) (H2 : s2 = t2) :
+  lam s0 s1 s2 = lam t0 t1 t2.
 Proof.
-exact (eq_trans (eq_trans eq_refl (ap (fun x => lam x s1) H0))
-         (ap (fun x => lam t0 x) H1)).
+exact (eq_trans
+         (eq_trans (eq_trans eq_refl (ap (fun x => lam x s1 s2) H0))
+            (ap (fun x => lam t0 x s2) H1)) (ap (fun x => lam t0 t1 x) H2)).
 Qed.
 
 Lemma congr_app {s0 : term} {s1 : term} {t0 : term} {t1 : term}
@@ -135,8 +137,8 @@ Fixpoint ren_term (xi_term : nat -> nat) (s : term) {struct s} : term :=
   | Sort s0 s1 => Sort s0 s1
   | Pi s0 s1 s2 s3 =>
       Pi s0 s1 (ren_term xi_term s2) (ren_term (upRen_term_term xi_term) s3)
-  | lam s0 s1 =>
-      lam (ren_term xi_term s0) (ren_term (upRen_term_term xi_term) s1)
+  | lam s0 s1 s2 =>
+      lam s0 (ren_term xi_term s1) (ren_term (upRen_term_term xi_term) s2)
   | app s0 s1 => app (ren_term xi_term s0) (ren_term xi_term s1)
   | Erased s0 => Erased (ren_term xi_term s0)
   | erase s0 => erase (ren_term xi_term s0)
@@ -168,9 +170,9 @@ term :=
   | Pi s0 s1 s2 s3 =>
       Pi s0 s1 (subst_term sigma_term s2)
         (subst_term (up_term_term sigma_term) s3)
-  | lam s0 s1 =>
-      lam (subst_term sigma_term s0)
-        (subst_term (up_term_term sigma_term) s1)
+  | lam s0 s1 s2 =>
+      lam s0 (subst_term sigma_term s1)
+        (subst_term (up_term_term sigma_term) s2)
   | app s0 s1 => app (subst_term sigma_term s0) (subst_term sigma_term s1)
   | Erased s0 => Erased (subst_term sigma_term s0)
   | erase s0 => erase (subst_term sigma_term s0)
@@ -211,9 +213,9 @@ subst_term sigma_term s = s :=
   | Pi s0 s1 s2 s3 =>
       congr_Pi (eq_refl s0) (eq_refl s1) (idSubst_term sigma_term Eq_term s2)
         (idSubst_term (up_term_term sigma_term) (upId_term_term _ Eq_term) s3)
-  | lam s0 s1 =>
-      congr_lam (idSubst_term sigma_term Eq_term s0)
-        (idSubst_term (up_term_term sigma_term) (upId_term_term _ Eq_term) s1)
+  | lam s0 s1 s2 =>
+      congr_lam (eq_refl s0) (idSubst_term sigma_term Eq_term s1)
+        (idSubst_term (up_term_term sigma_term) (upId_term_term _ Eq_term) s2)
   | app s0 s1 =>
       congr_app (idSubst_term sigma_term Eq_term s0)
         (idSubst_term sigma_term Eq_term s1)
@@ -264,10 +266,10 @@ ren_term xi_term s = ren_term zeta_term s :=
         (extRen_term xi_term zeta_term Eq_term s2)
         (extRen_term (upRen_term_term xi_term) (upRen_term_term zeta_term)
            (upExtRen_term_term _ _ Eq_term) s3)
-  | lam s0 s1 =>
-      congr_lam (extRen_term xi_term zeta_term Eq_term s0)
+  | lam s0 s1 s2 =>
+      congr_lam (eq_refl s0) (extRen_term xi_term zeta_term Eq_term s1)
         (extRen_term (upRen_term_term xi_term) (upRen_term_term zeta_term)
-           (upExtRen_term_term _ _ Eq_term) s1)
+           (upExtRen_term_term _ _ Eq_term) s2)
   | app s0 s1 =>
       congr_app (extRen_term xi_term zeta_term Eq_term s0)
         (extRen_term xi_term zeta_term Eq_term s1)
@@ -319,10 +321,10 @@ subst_term sigma_term s = subst_term tau_term s :=
         (ext_term sigma_term tau_term Eq_term s2)
         (ext_term (up_term_term sigma_term) (up_term_term tau_term)
            (upExt_term_term _ _ Eq_term) s3)
-  | lam s0 s1 =>
-      congr_lam (ext_term sigma_term tau_term Eq_term s0)
+  | lam s0 s1 s2 =>
+      congr_lam (eq_refl s0) (ext_term sigma_term tau_term Eq_term s1)
         (ext_term (up_term_term sigma_term) (up_term_term tau_term)
-           (upExt_term_term _ _ Eq_term) s1)
+           (upExt_term_term _ _ Eq_term) s2)
   | app s0 s1 =>
       congr_app (ext_term sigma_term tau_term Eq_term s0)
         (ext_term sigma_term tau_term Eq_term s1)
@@ -374,11 +376,12 @@ Fixpoint compRenRen_term (xi_term : nat -> nat) (zeta_term : nat -> nat)
         (compRenRen_term (upRen_term_term xi_term)
            (upRen_term_term zeta_term) (upRen_term_term rho_term)
            (up_ren_ren _ _ _ Eq_term) s3)
-  | lam s0 s1 =>
-      congr_lam (compRenRen_term xi_term zeta_term rho_term Eq_term s0)
+  | lam s0 s1 s2 =>
+      congr_lam (eq_refl s0)
+        (compRenRen_term xi_term zeta_term rho_term Eq_term s1)
         (compRenRen_term (upRen_term_term xi_term)
            (upRen_term_term zeta_term) (upRen_term_term rho_term)
-           (up_ren_ren _ _ _ Eq_term) s1)
+           (up_ren_ren _ _ _ Eq_term) s2)
   | app s0 s1 =>
       congr_app (compRenRen_term xi_term zeta_term rho_term Eq_term s0)
         (compRenRen_term xi_term zeta_term rho_term Eq_term s1)
@@ -437,11 +440,12 @@ subst_term tau_term (ren_term xi_term s) = subst_term theta_term s :=
         (compRenSubst_term (upRen_term_term xi_term) (up_term_term tau_term)
            (up_term_term theta_term) (up_ren_subst_term_term _ _ _ Eq_term)
            s3)
-  | lam s0 s1 =>
-      congr_lam (compRenSubst_term xi_term tau_term theta_term Eq_term s0)
+  | lam s0 s1 s2 =>
+      congr_lam (eq_refl s0)
+        (compRenSubst_term xi_term tau_term theta_term Eq_term s1)
         (compRenSubst_term (upRen_term_term xi_term) (up_term_term tau_term)
            (up_term_term theta_term) (up_ren_subst_term_term _ _ _ Eq_term)
-           s1)
+           s2)
   | app s0 s1 =>
       congr_app (compRenSubst_term xi_term tau_term theta_term Eq_term s0)
         (compRenSubst_term xi_term tau_term theta_term Eq_term s1)
@@ -511,12 +515,12 @@ ren_term zeta_term (subst_term sigma_term s) = subst_term theta_term s :=
         (compSubstRen_term (up_term_term sigma_term)
            (upRen_term_term zeta_term) (up_term_term theta_term)
            (up_subst_ren_term_term _ _ _ Eq_term) s3)
-  | lam s0 s1 =>
-      congr_lam
-        (compSubstRen_term sigma_term zeta_term theta_term Eq_term s0)
+  | lam s0 s1 s2 =>
+      congr_lam (eq_refl s0)
+        (compSubstRen_term sigma_term zeta_term theta_term Eq_term s1)
         (compSubstRen_term (up_term_term sigma_term)
            (upRen_term_term zeta_term) (up_term_term theta_term)
-           (up_subst_ren_term_term _ _ _ Eq_term) s1)
+           (up_subst_ren_term_term _ _ _ Eq_term) s2)
   | app s0 s1 =>
       congr_app
         (compSubstRen_term sigma_term zeta_term theta_term Eq_term s0)
@@ -595,12 +599,12 @@ subst_term tau_term (subst_term sigma_term s) = subst_term theta_term s :=
         (compSubstSubst_term (up_term_term sigma_term)
            (up_term_term tau_term) (up_term_term theta_term)
            (up_subst_subst_term_term _ _ _ Eq_term) s3)
-  | lam s0 s1 =>
-      congr_lam
-        (compSubstSubst_term sigma_term tau_term theta_term Eq_term s0)
+  | lam s0 s1 s2 =>
+      congr_lam (eq_refl s0)
+        (compSubstSubst_term sigma_term tau_term theta_term Eq_term s1)
         (compSubstSubst_term (up_term_term sigma_term)
            (up_term_term tau_term) (up_term_term theta_term)
-           (up_subst_subst_term_term _ _ _ Eq_term) s1)
+           (up_subst_subst_term_term _ _ _ Eq_term) s2)
   | app s0 s1 =>
       congr_app
         (compSubstSubst_term sigma_term tau_term theta_term Eq_term s0)
@@ -730,10 +734,10 @@ Fixpoint rinst_inst_term (xi_term : nat -> nat) (sigma_term : nat -> term)
         (rinst_inst_term xi_term sigma_term Eq_term s2)
         (rinst_inst_term (upRen_term_term xi_term) (up_term_term sigma_term)
            (rinstInst_up_term_term _ _ Eq_term) s3)
-  | lam s0 s1 =>
-      congr_lam (rinst_inst_term xi_term sigma_term Eq_term s0)
+  | lam s0 s1 s2 =>
+      congr_lam (eq_refl s0) (rinst_inst_term xi_term sigma_term Eq_term s1)
         (rinst_inst_term (upRen_term_term xi_term) (up_term_term sigma_term)
-           (rinstInst_up_term_term _ _ Eq_term) s1)
+           (rinstInst_up_term_term _ _ Eq_term) s2)
   | app s0 s1 =>
       congr_app (rinst_inst_term xi_term sigma_term Eq_term s0)
         (rinst_inst_term xi_term sigma_term Eq_term s1)
@@ -966,9 +970,10 @@ Fixpoint allfv_term (p_term : nat -> Prop) (s : term) {struct s} : Prop :=
         (and True
            (and (allfv_term p_term s2)
               (and (allfv_term (upAllfv_term_term p_term) s3) True)))
-  | lam s0 s1 =>
-      and (allfv_term p_term s0)
-        (and (allfv_term (upAllfv_term_term p_term) s1) True)
+  | lam s0 s1 s2 =>
+      and True
+        (and (allfv_term p_term s1)
+           (and (allfv_term (upAllfv_term_term p_term) s2) True))
   | app s0 s1 => and (allfv_term p_term s0) (and (allfv_term p_term s1) True)
   | Erased s0 => and (allfv_term p_term s0) True
   | erase s0 => and (allfv_term p_term s0) True
@@ -1011,11 +1016,12 @@ Fixpoint allfvTriv_term (p_term : nat -> Prop) (H_term : forall x, p_term x)
               (conj
                  (allfvTriv_term (upAllfv_term_term p_term)
                     (upAllfvTriv_term_term H_term) s3) I)))
-  | lam s0 s1 =>
-      conj (allfvTriv_term p_term H_term s0)
-        (conj
-           (allfvTriv_term (upAllfv_term_term p_term)
-              (upAllfvTriv_term_term H_term) s1) I)
+  | lam s0 s1 s2 =>
+      conj I
+        (conj (allfvTriv_term p_term H_term s1)
+           (conj
+              (allfvTriv_term (upAllfv_term_term p_term)
+                 (upAllfvTriv_term_term H_term) s2) I))
   | app s0 s1 =>
       conj (allfvTriv_term p_term H_term s0)
         (conj (allfvTriv_term p_term H_term s1) I)
@@ -1092,21 +1098,27 @@ allfv_term p_term s -> allfv_term q_term s :=
                             end
                         end
                     end) I)))
-  | lam s0 s1 =>
+  | lam s0 s1 s2 =>
       fun HP =>
-      conj
-        (allfvImpl_term p_term q_term H_term s0
-           match HP with
-           | conj HP _ => HP
-           end)
+      conj I
         (conj
-           (allfvImpl_term (upAllfv_term_term p_term)
-              (upAllfv_term_term q_term) (upAllfvImpl_term_term H_term) s1
+           (allfvImpl_term p_term q_term H_term s1
               match HP with
               | conj _ HP => match HP with
                              | conj HP _ => HP
                              end
-              end) I)
+              end)
+           (conj
+              (allfvImpl_term (upAllfv_term_term p_term)
+                 (upAllfv_term_term q_term) (upAllfvImpl_term_term H_term) s2
+                 match HP with
+                 | conj _ HP =>
+                     match HP with
+                     | conj _ HP => match HP with
+                                    | conj HP _ => HP
+                                    end
+                     end
+                 end) I))
   | app s0 s1 =>
       fun HP =>
       conj
@@ -1306,21 +1318,28 @@ allfv_term (funcomp p_term xi_term) s :=
                                end
                            end
                        end)) I)))
-  | lam s0 s1 =>
+  | lam s0 s1 s2 =>
       fun H =>
-      conj
-        (allfvRenL_term p_term xi_term s0 match H with
-                                          | conj H _ => H
-                                          end)
+      conj I
         (conj
-           (allfvImpl_term _ _ (upAllfvRenL_term_term p_term xi_term) s1
-              (allfvRenL_term (upAllfv_term_term p_term)
-                 (upRen_term_term xi_term) s1
-                 match H with
-                 | conj _ H => match H with
-                               | conj H _ => H
-                               end
-                 end)) I)
+           (allfvRenL_term p_term xi_term s1
+              match H with
+              | conj _ H => match H with
+                            | conj H _ => H
+                            end
+              end)
+           (conj
+              (allfvImpl_term _ _ (upAllfvRenL_term_term p_term xi_term) s2
+                 (allfvRenL_term (upAllfv_term_term p_term)
+                    (upRen_term_term xi_term) s2
+                    match H with
+                    | conj _ H =>
+                        match H with
+                        | conj _ H => match H with
+                                      | conj H _ => H
+                                      end
+                        end
+                    end)) I))
   | app s0 s1 =>
       fun H =>
       conj
@@ -1512,21 +1531,29 @@ allfv_term p_term (ren_term xi_term s) :=
                                end
                            end
                        end)) I)))
-  | lam s0 s1 =>
+  | lam s0 s1 s2 =>
       fun H =>
-      conj
-        (allfvRenR_term p_term xi_term s0 match H with
-                                          | conj H _ => H
-                                          end)
+      conj I
         (conj
-           (allfvRenR_term (upAllfv_term_term p_term)
-              (upRen_term_term xi_term) s1
-              (allfvImpl_term _ _ (upAllfvRenR_term_term p_term xi_term) s1
-                 match H with
-                 | conj _ H => match H with
-                               | conj H _ => H
-                               end
-                 end)) I)
+           (allfvRenR_term p_term xi_term s1
+              match H with
+              | conj _ H => match H with
+                            | conj H _ => H
+                            end
+              end)
+           (conj
+              (allfvRenR_term (upAllfv_term_term p_term)
+                 (upRen_term_term xi_term) s2
+                 (allfvImpl_term _ _ (upAllfvRenR_term_term p_term xi_term)
+                    s2
+                    match H with
+                    | conj _ H =>
+                        match H with
+                        | conj _ H => match H with
+                                      | conj H _ => H
+                                      end
+                        end
+                    end)) I))
   | app s0 s1 =>
       fun H =>
       conj
